src/Ring.fst
@@ -13,38 +13,12 @@ open FStar.Seq
 
 
 
-
-//abstract noeq
-//type ringstruct a = { rbuf: B.buffer a; head: UInt32.t; tail: UInt32.t; rsize: UInt32.t}
-
-abstract noeq
-type ringstruct a = { rbuf: B.buffer a; headptr: B.pointer UInt32.t; tailptr: B.pointer UInt32.t; rsize: UInt32.t}
-
-
 let is_rb_full (rsize:UInt32.t) (head:UInt32.t {UInt32.lt head rsize}) (tail:UInt32.t{ UInt32.lt tail rsize}) : Tot bool
   = (UInt32.add head 1ul) = tail
 
 let is_rb_empty (rsize:UInt32.t) (head:UInt32.t {UInt32.lt head rsize}) (tail:UInt32.t {UInt32.lt tail rsize}) : Tot bool
   = UInt32.eq head tail
 
-let live_rb (#a:eqtype) (h:HS.mem) (r:ringstruct a) : GTot Type0
-= B.live h r.rbuf
-/\ B.live h r.headptr
-/\ B.live h r.tailptr
-/\ loc_disjoint (loc_buffer r.rbuf) (loc_buffer r.headptr)
-/\ loc_disjoint (loc_buffer r.rbuf) (loc_buffer r.tailptr)
-/\ loc_disjoint (loc_buffer r.headptr) (loc_buffer r.tailptr)
-
-let well_formed_rb (#a:eqtype) (h:HS.mem) (r:ringstruct a): GTot bool
-  = 
-  let head = B.get h r.headptr 0 in
-  let tail = B.get h r.tailptr 0 in
-  UInt32.lt head r.rsize && 
-  UInt32.lt tail r.rsize &&
-  B.length r.rbuf = UInt32.v r.rsize &&
-  B.length r.rbuf > 0
-//  B.length r.headptr = 1 &&
-//  B.length r.tailptr = 1
 
 
 let incr_ht_spec (ht:UInt32.t) (rsize:UInt32.t{ UInt32.lt ht rsize}) : GTot  (l:UInt32.t {UInt32.lt l rsize})
@@ -55,17 +29,6 @@ let incr_ht_spec (ht:UInt32.t) (rsize:UInt32.t{ UInt32.lt ht rsize}) : GTot  (l:
   else ht'
 
 
-
-let get_head_spec (#a:eqtype) (h:HS.mem) (r:ringstruct a {well_formed_rb h r}): GTot (r':UInt32.t {UInt32.lt r' r.rsize})
-= B.get h r.headptr 0
-
-let get_tail_spec (#a:eqtype) (h:HS.mem) (r:ringstruct a {well_formed_rb h r}): GTot (r':UInt32.t {UInt32.lt r' r.rsize})
-= B.get h r.tailptr 0
-
-//increment the head by 1 push
-let incr_head_spec (#a:eqtype) (h:HS.mem) (r:ringstruct a {well_formed_rb h r}): GTot (r':UInt32.t {UInt32.lt r' r.rsize})
- = let head = B.get h r.headptr 0 in
-  incr_ht_spec head r.rsize
 
 //increment the head by 2 push
 let incr2_head_spec (#a:eqtype) (h:HS.mem) (r:ringstruct a {well_formed_rb h r /\ (UInt32.gt r.rsize 2ul)}): GTot (r':UInt32.t {UInt32.lt r' r.rsize})
@@ -122,67 +85,6 @@ let ht1 = UInt32.add ht 1ul in
                else ht4
   
 
-let incr_tail_spec (#a:eqtype) (h:HS.mem) (r:ringstruct a {well_formed_rb h r}): GTot (r':UInt32.t {UInt32.lt r' r.rsize})
-  = let tail = B.get h r.tailptr 0 in
-  incr_ht_spec tail r.rsize
-
-let incr2_tail_spec (#a:eqtype) (h:HS.mem) (r:ringstruct a {well_formed_rb h r /\ (UInt32.gt r.rsize 2ul)}): GTot (r':UInt32.t {UInt32.lt r' r.rsize})
-=
-let ht = B.get h r.tailptr 0 in
-let rsize = r.rsize in
-let _ = assert(UInt32.lt ht rsize) in
-let ht1 = UInt32.add ht 1ul in
-  if (UInt32.eq ht1 rsize) then 1ul
-  else
-    let _ = assert(UInt32.lt ht1 rsize) in
-    let ht2 = UInt32.add ht1 1ul in
-       if (UInt32.eq ht2 rsize)  then 0ul
-         else ht2
-
-let incr3_tail_spec (#a:eqtype) (h:HS.mem) (r:ringstruct a {well_formed_rb h r /\ (UInt32.gt r.rsize 3ul)}): GTot (r':UInt32.t {UInt32.lt r' r.rsize})
-=
-let ht = B.get h r.tailptr 0 in
-let rsize = r.rsize in
-let _ = assert(UInt32.lt ht rsize) in
-let ht1 = UInt32.add ht 1ul in
-  if (UInt32.eq ht1 rsize) then 2ul
-  else
-    let _ = assert(UInt32.lt ht1 rsize) in
-    let ht2 = UInt32.add ht1 1ul in
-       if (UInt32.eq ht2 rsize)  then 1ul
-         else 
-           let _ = assert(UInt32.lt ht2 rsize) in
-           let ht3 = UInt32.add ht2 1ul in
-           if (UInt32.eq ht3 rsize)  then 0ul
-             else ht3
-
-let incr4_tail_spec (#a:eqtype) (h:HS.mem) (r:ringstruct a {well_formed_rb h r /\ (UInt32.gt r.rsize 4ul)}): GTot (r':UInt32.t {UInt32.lt r' r.rsize})
-=
-let ht = B.get h r.tailptr 0 in
-let rsize = r.rsize in
-let _ = assert(UInt32.lt ht rsize) in
-let ht1 = UInt32.add ht 1ul in
-  if (UInt32.eq ht1 rsize) then 3ul
-  else
-    let _ = assert(UInt32.lt ht1 rsize) in
-    let ht2 = UInt32.add ht1 1ul in
-       if (UInt32.eq ht2 rsize)  then 2ul
-         else 
-           let _ = assert(UInt32.lt ht2 rsize) in
-           let ht3 = UInt32.add ht2 1ul in
-           if (UInt32.eq ht3 rsize)  then 1ul
-             else 
-               let _ = assert(UInt32.lt ht3 rsize) in
-               let ht4 = UInt32.add ht3 1ul in
-               if (UInt32.eq ht4 rsize) then 0ul
-               else ht4
-  
-
-let tail_unmodified_spec (#a:eqtype) (h0:HS.mem) (h1:HS.mem) (r0:ringstruct a) (r1: ringstruct a) : GTot bool
- = UInt32.eq (B.get h0 r0.tailptr 0) (B.get h1 r1.tailptr 0) 
-
-let head_unmodified_spec (#a:eqtype) (h0:HS.mem) (h1:HS.mem) (r0:ringstruct a) (r1: ringstruct a) : GTot bool
- = UInt32.eq (B.get h0 r0.headptr 0) (B.get h1 r1.headptr 0) 
 
 let rsize_unmodified_spec (#a:eqtype) (r0:ringstruct a) (r1: ringstruct a) : GTot bool
  = UInt32.eq r0.rsize r1.rsize 
@@ -194,24 +96,6 @@ let incr_ht (ht:UInt32.t) (rsize:UInt32.t{UInt32.lt ht rsize}) : Tot  (i:UInt32.
   if UInt32.eq ht' rsize then 0ul
   else ht'
 
-
-
-let get_current_size (head:UInt32.t) (tail:UInt32.t) (rsize:UInt32.t{UInt32.lt head rsize /\ UInt32.lt tail rsize}) : Tot  (i:UInt32.t {UInt32.lte i rsize})
- =
-  (*
-   *  ----------------------
-   *  |  |  |  |  |  |  |  | 
-   *  ----------------------
-   *   t        h
-   *  ----------------------
-   *  |  |  |  |  |  |  |  | 
-   *  ----------------------
-   *      h     t
-   *)
-   if (UInt32.gte head  tail) then (UInt32.sub head tail)
-   else //  (UInt32.lt head  tail)
-   (UInt32.sub rsize (UInt32.sub tail head))
-   
 
 let get_remaining_space (head:UInt32.t) (tail:UInt32.t) (rsize:UInt32.t{UInt32.lt head rsize /\ UInt32.lt tail rsize}) : Tot  (i:UInt32.t {UInt32.lte i rsize})
  =
@@ -228,13 +112,6 @@ let get_remaining_space (head:UInt32.t) (tail:UInt32.t) (rsize:UInt32.t{UInt32.l
    let c = get_current_size head tail rsize in
      (UInt32.sub rsize c)
    
-let get_current_size_spec (#a:eqtype) (h:HS.mem) (r:ringstruct a {well_formed_rb h r}) : GTot (i:UInt32.t {UInt32.lte i r.rsize})
-= 
-let head = B.get h r.headptr 0 in
-let tail = B.get h r.tailptr 0 in
-let rsize = r.rsize in
-get_current_size head tail rsize
-
 
 let remaining_space_spec (#a:eqtype) (h:HS.mem) (r:ringstruct a{well_formed_rb h r}): GTot  (r':UInt32.t {UInt32.lte r' r.rsize})
  =
@@ -260,38 +137,11 @@ let is_rb_empty_spec (#a:eqtype) (h:HS.mem) (r:ringstruct a {well_formed_rb h r}
   (UInt32.eq sz 0ul)
 
 
-let is_poppable (#a:eqtype) (r:ringstruct a): ST bool
-(requires fun h -> live_rb h r
-                /\ well_formed_rb h r
-)
-(ensures fun h0 s h1 -> live_rb h1 r
-                     /\ well_formed_rb h1 r
-                     /\ modifies loc_none h0 h1
-                     /\ ((s == true) ==>  not (is_rb_empty_spec h1 r))
-)
-= let head = !* r.headptr in
-let tail = !* r.tailptr in
-let rsize = r.rsize in
-let space = get_current_size head tail rsize in
-if (UInt32.gt space 0ul) then true
-else false
 
-let is_dword_poppable (#a:eqtype) (r:ringstruct a): ST bool
-(requires fun h -> live_rb h r
-                /\ well_formed_rb h r
-)
-(ensures fun h0 s h1 -> live_rb h1 r
-                     /\ well_formed_rb h1 r
-                     /\ modifies loc_none h0 h1
-                     /\ ((s == true) ==>  (UInt32.gte (get_current_size_spec h1 r) 4ul))
-)
-= let head = !* r.headptr in
-let tail = !* r.tailptr in
-let rsize = r.rsize in
-let space = get_current_size head tail rsize in
-if (UInt32.gte space 4ul) then true
-else false
-
+//increment the head by 1 push
+let incr_head_spec (#a:eqtype) (h:HS.mem) (r:ringstruct a {well_formed_rb h r}): GTot (r':UInt32.t {UInt32.lt r' r.rsize})
+ = let head = B.get h r.headptr 0 in
+  incr_ht_spec head r.rsize
 
 (* push: pushes an element at the head position
  * The pre-condition says that the invariants of the ringbuffer, namely,
@@ -332,7 +182,6 @@ let push (#a:eqtype) (r: ringstruct a) (v: a) : ST unit
 let push2 (#a:eqtype) (r: ringstruct a) (v1:a) (v2:a) : ST unit
   (requires fun h -> live_rb h r
                   /\  well_formed_rb h r
-//                  /\ not (is_rb_full_spec h r)
                      /\ UInt32.gt (remaining_space_spec h r) 4ul
                      /\ (UInt32.gt r.rsize 4ul)
                    )
@@ -343,7 +192,6 @@ let push2 (#a:eqtype) (r: ringstruct a) (v1:a) (v2:a) : ST unit
                     /\ well_formed_rb h1 r
                     /\ as_seq h1 r.rbuf == (Seq.upd (Seq.upd (as_seq h0 r.rbuf) (UInt32.v (get_head_spec h0 r)) v1)  (UInt32.v (incr_head_spec h0 r)) v2)
                     /\  get_head_spec h1 r == incr2_head_spec h0 r
-//                    /\ not (is_rb_empty_spec h1 r)
                     )
   =
   push r v1;
@@ -375,11 +223,12 @@ let push4 (#a:eqtype) (r: ringstruct a) (v1:a) (v2:a) (v3:a) (v4:a) : ST unit
   push r v4
 
 *)
-noeq
-type option 'a =
- | Error : option 'a
- | Value : v:'a -> option 'a
- 
+
+let incr_tail_spec (#a:eqtype) (h:HS.mem) (r:ringstruct a {well_formed_rb h r}): GTot (r':UInt32.t {UInt32.lt r' r.rsize})
+  = let tail = B.get h r.tailptr 0 in
+  incr_ht_spec tail r.rsize
+
+
 (* pop:  pop off the element at tail
  * The pre-condition checks that the invariants of the ringbuffer hold while
  * the post-condition says that the element read from the ringbuffer is same as the 
@@ -412,6 +261,24 @@ let pop (#a:eqtype) (r: ringstruct a) : ST a
   B.index r.rbuf tail
 
 
+// Check if the ring buffer can be popped.
+// Used by clients
+let is_poppable (#a:eqtype) (r:ringstruct a)
+= let head = !* r.headptr in
+let tail = !* r.tailptr in
+let rsize = r.rsize in
+let space = get_current_size head tail rsize in
+if (UInt32.gt space 0ul) then true
+else false
+
+let is_dword_poppable (#a:eqtype) (r:ringstruct a)
+= let head = !* r.headptr in
+let tail = !* r.tailptr in
+let rsize = r.rsize in
+let space = get_current_size head tail rsize in
+if (UInt32.gte space 4ul) then true
+else false
+
 
 #set-options "--z3rlimit 80 --initial_fuel 1 --max_fuel 1"
 //Handy routines
@@ -440,7 +307,11 @@ let pop4 (#a:eqtype) (r: ringstruct a) : ST (a*a*a*a)
    let m3 = pop r in
    let m4 = pop r in
    (m1, m2, m3, m4)
-   
+
+
+
+
+
 // The way the fullness of ringbuffer is checked requires that the minimum size is 2
 let init (#a:eqtype) (i: a) (s:UInt32.t {UInt32.gt s 1ul}) (hid: HS.rid) : ST (ringstruct a)
 (requires fun h -> true
@@ -473,17 +344,7 @@ let rlen = 32ul in
   let rinit = 1uy in
   //ringbuffer is located in host memory region but is disjoint from the host_memory
   let rb = init rinit rlen HS.root in
-//  let h' = HST.get () in
-//  assert(live_rb h' rb);
-//  assert(not (is_rb_full_spec h' rb));
   let _ = push rb 3uy in
-//  let h'' = HST.get () in
-//  assert(B.live h'' rb.headptr);
-//  assert(not (is_rb_empty_spec h'' rb));
- // let hd = !* (rb.headptr) in
-//  assert(B.live h'' rb.headptr);
-//  assert((B.get h'' rb.headptr 0) = (incr_head_spec h' rb));
-//  assert(hd = (incr_head_spec h' rb));
   let _ = pop rb in  
   let _ = push rb 4uy in
   let v = pop rb in
