src/Reader.fst
@@ -58,6 +58,6 @@ abstract let read (r: ringstruct8) (f:message -> datapointer  -> m_size_t -> UIn
     s
     else 0ul
   else
-     0ul
+    0ul
      
 
