src/Ring.fsti
@@ -1,0 +1,259 @@
+module Ring
+
+module B = LowStar.Buffer
+module HS = FStar.HyperStack
+module HST = FStar.HyperStack.ST
+module U64 =   FStar.UInt64
+module I8 =   FStar.Int8
+module U8 =   FStar.UInt8
+open LowStar.BufferOps
+open FStar.HyperStack.ST
+include LowStar.Monotonic.Buffer
+open FStar.Seq
+
+
+abstract noeq
+type ringstruct a = { rbuf: B.buffer a; headptr: B.pointer UInt32.t; tailptr: B.pointer UInt32.t; rsize: UInt32.t}
+
+//val live_rb: (#a:eqtype)->(h:HS.mem)->(r:ringstruct a)->GTot Type0
+let live_rb (#a:eqtype) (h:HS.mem) (r:ringstruct a) : GTot Type0
+= B.live h r.rbuf
+/\ B.live h r.headptr
+/\ B.live h r.tailptr
+/\ loc_disjoint (loc_buffer r.rbuf) (loc_buffer r.headptr)
+/\ loc_disjoint (loc_buffer r.rbuf) (loc_buffer r.tailptr)
+/\ loc_disjoint (loc_buffer r.headptr) (loc_buffer r.tailptr)
+
+
+let well_formed_rb (#a:eqtype) (h:HS.mem) (r:ringstruct a): GTot bool
+  = 
+  let head = B.get h r.headptr 0 in
+  let tail = B.get h r.tailptr 0 in
+  UInt32.lt head r.rsize && 
+  UInt32.lt tail r.rsize &&
+  B.length r.rbuf = UInt32.v r.rsize &&
+  B.length r.rbuf > 0
+
+//val get_current_size: (head:UInt32.t)->(tail:UInt32.t)->(rsize:UInt32.t{UInt32.lt head rsize /\ UInt32.lt tail rsize})-> Tot  (i:UInt32.t {UInt32.lte i rsize})
+let get_current_size (head:UInt32.t) (tail:UInt32.t) (rsize:UInt32.t{UInt32.lt head rsize /\ UInt32.lt tail rsize}) : Tot  (i:UInt32.t {UInt32.lte i rsize})
+ =
+  (*
+   *  ----------------------
+   *  |  |  |  |  |  |  |  | 
+   *  ----------------------
+   *   t        h
+   *  ----------------------
+   *  |  |  |  |  |  |  |  | 
+   *  ----------------------
+   *      h     t
+   *)
+   if (UInt32.gte head  tail) then (UInt32.sub head tail)
+   else //  (UInt32.lt head  tail)
+   (UInt32.sub rsize (UInt32.sub tail head))
+
+//val get_current_size_spec: (#a:eqtype)->(h:HS.mem)->(r:ringstruct a {well_formed_rb h r})-> GTot (i:UInt32.t {UInt32.lte i r.rsize})
+let get_current_size_spec (#a:eqtype) (h:HS.mem) (r:ringstruct a {well_formed_rb h r}) : GTot (i:UInt32.t {UInt32.lte i r.rsize})
+= 
+let head = B.get h r.headptr 0 in
+let tail = B.get h r.tailptr 0 in
+let rsize = r.rsize in
+get_current_size head tail rsize
+
+
+//val tail_unmodified_spec: (#a:eqtype)->(h0:HS.mem)->(h1:HS.mem)->(r0:ringstruct a)->(r1: ringstruct a)->GTot bool
+let tail_unmodified_spec (#a:eqtype) (h0:HS.mem) (h1:HS.mem) (r0:ringstruct a) (r1: ringstruct a) : GTot bool
+ = UInt32.eq (B.get h0 r0.tailptr 0) (B.get h1 r1.tailptr 0) 
+
+
+val is_rb_full_spec: (#a:eqtype)->(h:HS.mem)->(r:ringstruct a {well_formed_rb h r})->GTot bool
+val is_rb_empty_spec: (#a:eqtype)->(h:HS.mem)->(r:ringstruct a {well_formed_rb h r})-> GTot bool
+
+
+let get_head_spec (#a:eqtype) (h:HS.mem) (r:ringstruct a {well_formed_rb h r}): GTot (r':UInt32.t {UInt32.lt r' r.rsize})
+= B.get h r.headptr 0
+
+//increment the head by 1 push
+val incr_head_spec: (#a:eqtype)->(h:HS.mem)->(r:ringstruct a {well_formed_rb h r})->GTot (r':UInt32.t {UInt32.lt r' r.rsize})
+
+
+
+(* push: pushes an element at the head position
+ * The pre-condition says that the invariants of the ringbuffer, namely,
+ * 1. head and tail are always less than the size of the buffer
+ * 2. size of the buffer is at least 1
+ * 3. Buffer is live
+ * hold. The post-condition says that if the 'push' is successful, then
+ * the resulting buffer in the new heap is same as the buffer in the old heap with the element
+ * pushed into the head position. If not, buffer remains the same.
+ * The post-condition also says that the invariants are preserved, and that the buffer is live.
+ *)
+val push:(#a:eqtype)->(r: ringstruct a)->(v: a) ->ST unit
+  (requires fun h -> live_rb h r
+                  /\  well_formed_rb h r
+                  /\ not (is_rb_full_spec h r)
+                   )
+  (ensures fun h0 _ h1 -> 
+                    live_rb h1 r 
+                    /\ modifies (loc_union (loc_buffer r.rbuf)  (loc_buffer r.headptr)) h0 h1
+                    /\ tail_unmodified_spec h0 h1 r r 
+                    /\ well_formed_rb h1 r
+                      /\ as_seq h1 r.rbuf == Seq.upd (as_seq h0 r.rbuf) (UInt32.v (get_head_spec h0 r)) v
+                      /\  get_head_spec h1 r == incr_head_spec h0 r
+                      /\ not (is_rb_empty_spec h1 r)
+                    )
+
+//val head_unmodified_spec: (#a:eqtype)->(h0:HS.mem)->(h1:HS.mem)->(r0:ringstruct a)->(r1: ringstruct a)->GTot bool
+
+let head_unmodified_spec (#a:eqtype) (h0:HS.mem) (h1:HS.mem) (r0:ringstruct a) (r1: ringstruct a) : GTot bool
+ = UInt32.eq (B.get h0 r0.headptr 0) (B.get h1 r1.headptr 0) 
+
+let get_tail_spec (#a:eqtype) (h:HS.mem) (r:ringstruct a {well_formed_rb h r}): GTot (r':UInt32.t {UInt32.lt r' r.rsize})
+= B.get h r.tailptr 0
+
+val incr_tail_spec: (#a:eqtype)->(h:HS.mem)->(r:ringstruct a {well_formed_rb h r})->GTot (r':UInt32.t {UInt32.lt r' r.rsize})
+
+ 
+(* pop:  pop off the element at tail
+ * The pre-condition checks that the invariants of the ringbuffer hold while
+ * the post-condition says that the element read from the ringbuffer is same as the 
+ * one read from the same index in the sequence formed from buffer. When the ringbuffer is full
+ * tail is not modified other tail is modified.
+ * The post-condition also says that the invariants are preserved
+ *)
+val pop:(#a:eqtype)->(r: ringstruct a)->ST a 
+  (requires fun h0 -> live_rb h0 r 
+                     /\ well_formed_rb h0 r
+                     /\ (UInt32.gt (get_current_size_spec h0 r) 0ul)
+                    )
+  (ensures fun h0 v h1 -> live_rb h1 r
+                   /\ well_formed_rb h1 r
+                   /\ modifies (loc_buffer r.tailptr) h0 h1
+                   /\ as_seq h1 r.rbuf == as_seq h0 r.rbuf
+                   /\ head_unmodified_spec h0 h1 r r 
+                   /\ (v == Seq.index (as_seq h1 r.rbuf) (UInt32.v (get_tail_spec h0 r)))
+                   /\ (get_tail_spec h1 r == incr_tail_spec h0 r)
+                   /\ (get_current_size_spec h1 r) = UInt32.sub (get_current_size_spec h0 r) 1ul
+  )
+
+
+
+//val incr2_tail_spec: (#a:eqtype)->(h:HS.mem)->(r:ringstruct a {well_formed_rb h r /\ (UInt32.gt r.rsize 2ul)})->GTot (r':UInt32.t {UInt32.lt r' r.rsize})
+let incr2_tail_spec (#a:eqtype) (h:HS.mem) (r:ringstruct a {well_formed_rb h r /\ (UInt32.gt r.rsize 3ul)}): GTot (r':UInt32.t {UInt32.lt r' r.rsize})
+=
+  let ht = B.get h r.tailptr 0 in
+  let rsize = r.rsize in
+  let _ = assert(UInt32.lt ht rsize) in
+  let ht1 = UInt32.add ht 1ul in
+    if (UInt32.eq ht1 rsize) then 1ul
+    else
+      let _ = assert(UInt32.lt ht1 rsize) in
+      let ht2 = UInt32.add ht1 1ul in
+        if (UInt32.eq ht2 rsize)  then 0ul
+          else ht2
+
+//val incr3_tail_spec: (#a:eqtype)->(h:HS.mem)->(r:ringstruct a {well_formed_rb h r /\ (UInt32.gt r.rsize 2ul)})->GTot (r':UInt32.t {UInt32.lt r' r.rsize})
+let incr3_tail_spec (#a:eqtype) (h:HS.mem) (r:ringstruct a {well_formed_rb h r /\ (UInt32.gt r.rsize 3ul)}): GTot (r':UInt32.t {UInt32.lt r' r.rsize})
+=
+let ht = B.get h r.tailptr 0 in
+let rsize = r.rsize in
+let _ = assert(UInt32.lt ht rsize) in
+let ht1 = UInt32.add ht 1ul in
+  if (UInt32.eq ht1 rsize) then 2ul
+  else
+    let _ = assert(UInt32.lt ht1 rsize) in
+    let ht2 = UInt32.add ht1 1ul in
+       if (UInt32.eq ht2 rsize)  then 1ul
+         else 
+           let _ = assert(UInt32.lt ht2 rsize) in
+           let ht3 = UInt32.add ht2 1ul in
+           if (UInt32.eq ht3 rsize)  then 0ul
+             else ht3
+
+//val incr4_tail_spec: (#a:eqtype)->(h:HS.mem)->(r:ringstruct a {well_formed_rb h r /\ (UInt32.gt r.rsize 2ul)})->GTot (r':UInt32.t {UInt32.lt r' r.rsize})
+let incr4_tail_spec (#a:eqtype) (h:HS.mem) (r:ringstruct a {well_formed_rb h r /\ (UInt32.gt r.rsize 4ul)}): GTot (r':UInt32.t {UInt32.lt r' r.rsize})
+=
+let ht = B.get h r.tailptr 0 in
+let rsize = r.rsize in
+let _ = assert(UInt32.lt ht rsize) in
+let ht1 = UInt32.add ht 1ul in
+  if (UInt32.eq ht1 rsize) then 3ul
+  else
+    let _ = assert(UInt32.lt ht1 rsize) in
+    let ht2 = UInt32.add ht1 1ul in
+       if (UInt32.eq ht2 rsize)  then 2ul
+         else 
+           let _ = assert(UInt32.lt ht2 rsize) in
+           let ht3 = UInt32.add ht2 1ul in
+           if (UInt32.eq ht3 rsize)  then 1ul
+             else 
+               let _ = assert(UInt32.lt ht3 rsize) in
+               let ht4 = UInt32.add ht3 1ul in
+               if (UInt32.eq ht4 rsize) then 0ul
+               else ht4
+
+
+// Check if the ring buffer can be popped.
+// Used by clients
+val is_poppable: (#a:eqtype)->(r:ringstruct a) ->ST bool
+(requires fun h -> live_rb h r
+                /\ well_formed_rb h r
+)
+(ensures fun h0 s h1 -> live_rb h1 r
+                     /\ well_formed_rb h1 r
+                     /\ modifies loc_none h0 h1
+//                     /\ ((s == true) ==>  not (is_rb_empty_spec h1 r))
+                       /\ ((s == true) ==>  (UInt32.gt (get_current_size_spec h1 r) 0ul))
+)
+
+// Check if the ring buffer can be popped 4 times.
+// Used by clients
+val is_dword_poppable: (#a:eqtype)->(r:ringstruct a)->ST bool
+(requires fun h -> live_rb h r
+                /\ well_formed_rb h r
+)
+(ensures fun h0 s h1 -> live_rb h1 r
+                     /\ well_formed_rb h1 r
+                     /\ modifies loc_none h0 h1
+                     /\ ((s == true) ==>  (UInt32.gte (get_current_size_spec h1 r) 4ul))
+)
+
+
+
+
+
+//Handy routines
+// Return a sequence of bytes
+//#set-options "--z3rlimit 80 --initial_fuel 1 --max_fuel 1"
+val pop4:(#a:eqtype)->(r: ringstruct a)->ST (a*a*a*a) 
+  (requires fun h0 -> live_rb h0 r 
+                     /\ well_formed_rb h0 r
+                     /\ UInt32.gte (get_current_size_spec h0 r) 4ul
+                    )
+  (ensures fun h0 (v1, v2, v3, v4) h1 -> live_rb h1 r
+                   /\ well_formed_rb h1 r
+                   /\ modifies (loc_buffer r.tailptr) h0 h1
+                   /\ as_seq h1 r.rbuf == as_seq h0 r.rbuf
+                   /\ head_unmodified_spec h0 h1 r r 
+                   /\ (v1 == Seq.index (as_seq h1 r.rbuf) (UInt32.v (get_tail_spec h0 r)))
+                   /\ (v2 == Seq.index (as_seq h1 r.rbuf) (UInt32.v (incr_tail_spec h0 r)))
+                   /\ (v3 == Seq.index (as_seq h1 r.rbuf) (UInt32.v (incr2_tail_spec h0 r)))
+                   /\ (v4 == Seq.index (as_seq h1 r.rbuf) (UInt32.v (incr3_tail_spec h0 r)))
+                   /\ (get_tail_spec h1 r == incr4_tail_spec h0 r)
+                   /\ (get_current_size_spec h0 r) = UInt32.add (get_current_size_spec h1 r) 4ul  
+  )
+
+// The way the fullness of ringbuffer is checked requires that the minimum size is 2
+val init: (#a:eqtype)->(i: a)->(s:UInt32.t {UInt32.gt s 1ul})->(hid: HS.rid)->ST (ringstruct a)
+(requires fun h -> true
+/\ is_eternal_region hid)
+(ensures fun h0 res h1 -> B.modifies B.loc_none h0 h1
+/\ B.fresh_loc (loc_buffer res.rbuf) h0 h1 
+/\ B.fresh_loc (loc_buffer res.headptr) h0 h1 
+/\ B.fresh_loc (loc_buffer res.tailptr) h0 h1 
+/\ well_formed_rb h1 res
+/\ live_rb h1 res
+/\ B.length res.rbuf == UInt32.v s
+/\ (is_rb_empty_spec h1 res)
+/\ not (is_rb_full_spec h1 res)
+/\ res.rsize = s
+)
